Correctness.thy
@@ -84,7 +84,7 @@ proof -
   moreover with R have R': "restructurable \<Sigma>\<^sub>u' ?cd" by fastforce
   moreover with EU obtain h\<^sub>u hp\<^sub>u e\<^sub>u ep\<^sub>u vs\<^sub>u vp\<^sub>u sh\<^sub>u where VU:
     "\<Sigma>\<^sub>u' = US h\<^sub>u hp\<^sub>u e\<^sub>u ep\<^sub>u vs\<^sub>u vp\<^sub>u sh\<^sub>u 0 0 \<and> flatten_values h\<^sub>c\<^sub>e = H h\<^sub>u hp\<^sub>u \<and> 
-      flatten_environment env\<^sub>h = H e\<^sub>u ep\<^sub>u \<and> listify' vs\<^sub>u vp\<^sub>u = 3 * v\<^sub>h # []" by auto
+      flatten_environment env\<^sub>h = H e\<^sub>u ep\<^sub>u \<and> listify_heap vs\<^sub>u vp\<^sub>u = 3 * v\<^sub>h # []" by auto
   moreover hence VSU: "vs\<^sub>u 0 = 3 * v\<^sub>h \<and> vp\<^sub>u = 1" by auto
   ultimately have "iter (\<tturnstile> ?cd \<leadsto>\<^sub>u) (US nmem 0 nmem 0 nmem 0 (nmem(0 := 0, 1 := 0)) 2 (length ?cd)) 
     (US h\<^sub>u hp\<^sub>u e\<^sub>u ep\<^sub>u vs\<^sub>u 1 sh\<^sub>u 0 0)" by simp
